cfrontend/Csem.v
@@ -38,7 +38,6 @@ Module Csem (P: Policy) (A: Allocator P).
 
   Import P.
   
-  
   (** * Operational semantics *)
 
   (** The semantics uses two environments.  The global environment
@@ -344,16 +343,21 @@ Module Csem (P: Policy) (A: Allocator P).
         e!x = Some (PUB base bound pt ty) ->
         lred (Evar x ty) pct te m
              (Eloc (Lmem (Int64.repr base) pt Full) ty) te m
-    | red_var_global: forall x ty pct lo hi pt gv te m,
+    | red_var_global: forall x ty pct base bound pt gv te m,
         e!x = None ->
-        Genv.find_symbol ge x = Some (inr (lo, hi, pt, gv)) ->
+        Genv.find_symbol ge x = Some (SymGlob base bound pt gv) ->
         lred (Evar x ty) pct te m
-             (Eloc (Lmem (Int64.repr lo) pt Full) ty) te m
+             (Eloc (Lmem (Int64.repr base) pt Full) ty) te m
     | red_func: forall x pct b pt ty te m,
         e!x = None ->
-        Genv.find_symbol ge x = Some (inl (b, pt)) ->
+        Genv.find_symbol ge x = Some (SymIFun _ b pt) ->
         lred (Evar x ty) pct te m
-             (Eloc (Lfun b pt) ty) te m
+             (Eloc (Lifun b pt) ty) te m
+    | red_ext_func: forall x pct ef tyargs tyres cc pt ty te m,
+        e!x = None ->
+        Genv.find_symbol ge x = Some (SymEFun _ ef tyargs tyres cc pt) ->
+        lred (Evar x ty) pct te m
+             (Eloc (Lefun ef tyargs tyres cc pt) ty) te m
     | red_deref_short: forall ofs vt ty1 ty pct te m,
         lred (Ederef (Eval (Vint ofs,vt) ty1) ty) pct te m
              (Eloc (Lmem (cast_int_long Unsigned ofs) vt Full) ty) te m
@@ -400,9 +404,12 @@ Module Csem (P: Policy) (A: Allocator P).
         AccessT PCT vt' = PolicySuccess vt'' ->
         rred PCT (Evalof (Eloc (Lmem ofs pt bf) ty) ty) te m tr
              PCT (Eval (v,vt'') ty) te m
-    | red_rvalof_fun: forall b pt ty te m,
-        rred PCT (Evalof (Eloc (Lfun b pt) ty) ty) te m E0
+    | red_rvalof_ifun: forall b pt ty te m,
+        rred PCT (Evalof (Eloc (Lifun b pt) ty) ty) te m E0
              PCT (Eval (Vfptr b, pt) ty) te m
+    | red_rvalof_efun: forall ef tyargs tyres cc pt ty te m,
+        rred PCT (Evalof (Eloc (Lefun ef tyargs tyres cc pt) ty) ty) te m E0
+             PCT (Eval (Vefptr ef tyargs tyres cc, pt) ty) te m
     | red_rvalof_tmp: forall b ty te m v vt vt',
         te!b = Some (v,vt) ->
         AccessT PCT vt = PolicySuccess vt' ->
@@ -412,8 +419,11 @@ Module Csem (P: Policy) (A: Allocator P).
         rred PCT (Eaddrof (Eloc (Lmem ofs pt Full) ty1) ty) te m E0
              PCT (Eval (Vlong ofs, pt) ty) te m
     | red_addrof_fptr: forall b pt ty te m,
-        rred PCT (Eaddrof (Eloc (Lfun b pt) ty) ty) te m E0
+        rred PCT (Eaddrof (Eloc (Lifun b pt) ty) ty) te m E0
              PCT (Eval (Vfptr b, pt) ty) te m
+    | red_addrof_efptr: forall ef tyargs tyres cc pt ty te m,
+        rred PCT (Eaddrof (Eloc (Lefun ef tyargs tyres cc pt) ty) ty) te m E0
+             PCT (Eval (Vefptr ef tyargs tyres cc, pt) ty) te m
     | red_unop: forall op v1 vt1 ty1 ty te m v PCT' vt,
         sem_unary_operation op v1 ty1 m = Some v ->
         UnopT op PCT vt1 = PolicySuccess (PCT', vt) ->
@@ -523,10 +533,14 @@ Module Csem (P: Policy) (A: Allocator P).
         rred PCT (Eassignop op (Eloc (Ltmp b) ty1) (Eval (v2,vt2) ty2) tyres ty1) te m E0
              PCT (Eassign (Eloc (Ltmp b) ty1)
                           (Ebinop op (Eval (v1,vt1') ty1) (Eval (v2,vt2) ty2) tyres) ty1) te m
-    | red_assignop_fun: forall op b pt ty1 v2 vt2 ty2 tyres te m,
-        rred PCT (Eassignop op (Eloc (Lfun b pt) ty1) (Eval (v2,vt2) ty2) tyres ty1) te m E0
-             PCT (Eassign (Eloc (Lfun b pt) ty1)
+    | red_assignop_ifun: forall op b pt ty1 v2 vt2 ty2 tyres te m,
+        rred PCT (Eassignop op (Eloc (Lifun b pt) ty1) (Eval (v2,vt2) ty2) tyres ty1) te m E0
+             PCT (Eassign (Eloc (Lifun b pt) ty1)
                           (Ebinop op (Eval (Vfptr b,pt) ty1) (Eval (v2,vt2) ty2) tyres) ty1) te m
+    | red_assignop_efun: forall op ef tyargs tyres cc pt ty1 v2 vt2 ty2 ty te m,
+        rred PCT (Eassignop op (Eloc (Lefun ef tyargs tyres cc pt) ty1) (Eval (v2,vt2) ty2) ty ty1) te m E0
+             PCT (Eassign (Eloc (Lefun ef tyargs tyres cc pt) ty1)
+                          (Ebinop op (Eval (Vefptr ef tyargs tyres cc,pt) ty1) (Eval (v2,vt2) ty2) ty) ty1) te m
     | red_postincr_mem: forall id ofs pt ty bf te m t v vt vt' vt'' lts op,
         deref_loc ty m ofs pt bf t (MemorySuccess ((v,vt), lts)) ->
         LoadT PCT pt vt lts = PolicySuccess vt' ->
@@ -550,15 +564,24 @@ Module Csem (P: Policy) (A: Allocator P).
                                           (incrdecr_type ty))
                                   ty)
                          (Eval (v,vt') ty) ty) te m
-    | red_postincr_fun: forall id b pt ty te m op,
+    | red_postincr_ifun: forall id b pt ty te m op,
         op = match id with Incr => Oadd | Decr => Osub end ->
-        rred PCT (Epostincr id (Eloc (Lfun b pt) ty) ty) te m E0
-             PCT (Ecomma (Eassign (Eloc (Lfun b pt) ty)
+        rred PCT (Epostincr id (Eloc (Lifun b pt) ty) ty) te m E0
+             PCT (Ecomma (Eassign (Eloc (Lifun b pt) ty)
                                   (Ebinop op (Eval (Vfptr b, pt) ty)
                                           (Econst (Vint Int.one) type_int32s)
                                           (incrdecr_type ty))
                                   ty)
                          (Eval (Vfptr b,pt) ty) ty) te m
+    | red_postincr_efun: forall id ef tyargs tyres cc pt ty te m op,
+        op = match id with Incr => Oadd | Decr => Osub end ->
+        rred PCT (Epostincr id (Eloc (Lefun ef tyargs tyres cc pt) ty) ty) te m E0
+             PCT (Ecomma (Eassign (Eloc (Lefun ef tyargs tyres cc pt) ty)
+                                  (Ebinop op (Eval (Vefptr ef tyargs tyres cc, pt) ty)
+                                          (Econst (Vint Int.one) type_int32s)
+                                          (incrdecr_type ty))
+                                  ty)
+                         (Eval (Vefptr ef tyargs tyres cc,pt) ty) ty) te m
     | red_comma: forall v ty1 r2 ty te m,
         typeof r2 = ty ->
         rred PCT (Ecomma (Eval v ty1) r2 ty) te m E0
@@ -567,11 +590,8 @@ Module Csem (P: Policy) (A: Allocator P).
         sem_cast v1 ty1 ty2 m = Some v ->
         ExprJoinT PCT vt1 = PolicySuccess (PCT', vt') ->
         rred PCT (Eparen (Eval (v1,vt1) ty1) ty2 ty) te m E0
-             PCT' (Eval (v,vt') ty) te m
-    | red_builtin: forall ef ty te m,
-        rred PCT (Ebuiltin ef ty) te m E0
-             PCT (Eval (Vefptr ef,def_tag) ty) te m.
-
+             PCT' (Eval (v,vt') ty) te m.
+    
     (** Failstops for r-values *)
     Inductive rfailred (PCT:tag) : expr -> tenv -> mem -> trace -> string -> FailureClass -> list tag -> Prop :=
     | failred_const: forall v ty te m msg params,
@@ -751,18 +771,16 @@ Module Csem (P: Policy) (A: Allocator P).
         (More exactly, identification of function calls that can reduce.) *)
     Inductive callred: tag -> expr -> mem -> fundef -> tag -> list atom -> type -> Prop :=
     | red_call_internal: forall PCT vf vft tyf m tyargs tyres cconv el ty fd vargs,
-        Genv.find_funct ge vf = Some (Internal fd) ->
+        Genv.find_funct ge vf = Some fd ->
         cast_arguments m el tyargs vargs ->
         type_of_fundef fd = Tfunction tyargs tyres cconv ->
         classify_fun tyf = fun_case_f tyargs tyres cconv ->
         callred PCT (Ecall (Eval (vf,vft) tyf) el ty) m
                 fd vft vargs ty
-    | red_call_external: forall PCT vf vft tyf m tyargs tyres cconv el ty ef vargs,
-        Genv.find_funct ge vf = Some (External ef tyargs tyres cconv) ->
+    | red_call_external: forall PCT vft tyf m tyargs tyres cconv el ty ef vargs,
         cast_arguments m el tyargs vargs ->
-        classify_fun tyf = fun_case_f tyargs tyres cconv ->
-        callred PCT (Ecall (Eval (vf,vft) tyf) el ty) m
-                (External ef tyargs tyres cconv) vft vargs ty.
+        callred PCT (Ecall (Eval (Vefptr ef tyargs tyres cconv,vft) tyf) el ty) m
+                (External ef tyargs ty cconv) vft vargs ty.
 
     (** Reduction contexts.  In accordance with C's nondeterministic semantics,
         we allow reduction both to the left and to the right of a binary operator.
@@ -1398,7 +1416,7 @@ End SEM.
   Inductive initial_state (p: program): state -> Prop :=
   | initial_state_intro: forall b pt f ge ce m0,
       globalenv p = MemorySuccess (ge,ce,m0) ->
-      Genv.find_symbol ge p.(prog_main) = Some (inl (b,pt)) ->
+      Genv.find_symbol ge p.(prog_main) = Some (SymIFun _ b pt) ->
       Genv.find_funct_ptr ge b = Some f ->
       type_of_fundef f = Tfunction Tnil type_int32s cc_default ->
       initial_state p (Callstate f InitPCT def_tag nil Kstop m0).
