common/Values.v
@@ -18,9 +18,10 @@
   semantics of all our intermediate languages. *)
 
 Require Import Coqlib.
-Require Import AST.
 Require Import Integers.
 Require Import Floats.
+Require Import Ctypes.
+Require Import AST.
 
 Definition block : Type := positive.
 Definition eq_block := peq.
@@ -41,7 +42,7 @@ Inductive val: Type :=
 | Vfloat: float -> val
 | Vsingle: float32 -> val
 | Vfptr: block -> val
-| Vefptr: external_function -> val
+| Vefptr: external_function -> typelist -> rettype -> calling_convention -> val
 .
 
 Definition Vzero: val := Vint Int.zero.
@@ -70,8 +71,13 @@ Proof.
   apply Float.eq_dec.
   apply Float32.eq_dec.
   apply eq_block.
+  repeat decide equality.
+  repeat decide equality.
+  decide equality.
+  apply type_eq.
   apply external_function_eq.
 Defined.
+
 Global Opaque eq.
 
 Definition has_type (v: val) (t: typ) : Prop :=
@@ -82,7 +88,7 @@ Definition has_type (v: val) (t: typ) : Prop :=
   | Vfloat _, Tfloat => True
   | Vsingle _, Tsingle => True
   | Vfptr _, Tlong => True
-  | Vefptr _, Tlong => True
+  | Vefptr _ _ _ _, Tlong => True
   | (Vint _ | Vsingle _), Tany32 => True
   | _, Tany64 => True
   | _, _ => False
@@ -894,7 +900,7 @@ Definition normalize (v: val) (ty: typ) : val :=
   | Vfloat _, Tfloat => v
   | Vsingle _, Tsingle => v
   | Vfptr _, Tlong => v
-  | Vefptr _, Tlong => v
+  | Vefptr _ _ _ _, Tlong => v
   | (Vint _ | Vsingle _), Tany32 => v
   | _, Tany64 => v
   | _, _ => Vundef
@@ -950,9 +956,9 @@ Definition load_result (chunk: memory_chunk) (v: val) :=
   | Mint16signed, Vint n => Vint (Int.sign_ext 16 n)
   | Mint16unsigned, Vint n => Vint (Int.zero_ext 16 n)
   | Mint32, Vint n => Vint n
-  | Mint64, Vlong n => Vlong n
-  | Mint64, Vfptr b => Vfptr b
-  | Mint64, Vefptr b => Vefptr b
+  | Mint64, Vlong _
+  | Mint64, Vfptr _
+  | Mint64, Vefptr _ _ _ _ => v 
   | Mfloat32, Vsingle f => Vsingle f
   | Mfloat64, Vfloat f => Vfloat f
   | Many32, (Vint _ | Vsingle _) => v
